src/ldrfra/RelWrites.v
@@ -1,0 +1,54 @@
+Require Import Omega.
+Require Import Bool.
+Require Import RelationClasses.
+
+From sflib Require Import sflib.
+From Paco Require Import paco.
+
+From PromisingLib Require Import Axioms.
+From PromisingLib Require Import Basic.
+From PromisingLib Require Import DataStructure.
+From PromisingLib Require Import DenseOrder.
+From PromisingLib Require Import Loc.
+From PromisingLib Require Import Language.
+
+Require Import Event.
+Require Import Time.
+Require Import View.
+Require Import Cell.
+Require Import Memory.
+Require Import MemoryFacts.
+Require Import TView.
+Require Import Local.
+
+Set Implicit Arguments.
+
+
+Module RelWrites.
+  Section RelWrites.
+    Variable L: Loc.t -> bool.
+
+    Definition t: Type := list (Loc.t * Time.t).
+
+    Definition append (e: ThreadEvent.t) (rels: t): t :=
+      match ThreadEvent.is_writing e with
+      | Some (loc, from, to, val, released, ord) =>
+        if L loc
+        then if Ordering.le Ordering.acqrel ord then (loc, to) :: rels else rels
+        else rels
+      | None => rels
+      end.
+
+    Definition wf (rels: t) (promises mem: Memory.t): Prop :=
+      forall loc to (IN: List.In (loc, to) rels),
+        Memory.get loc to promises = None /\
+        exists from val released,
+          Memory.get loc to mem = Some (from, Message.concrete val released).
+
+    Lemma append_app e rels1 rels2:
+      append e rels1 ++ rels2 = append e (rels1 ++ rels2).
+    Proof.
+      unfold append. des_ifs.
+    Qed.
+  End RelWrites.
+End RelWrites.
